Commit fully mutually recursive

Tealeaves/Examples/VariadicLet/Syntax.v
@@ -15,6 +15,8 @@ From Tealeaves Require Export
 #[local] Generalizable Variables G A B C.
 #[local] Set Implicit Arguments.
 
+Open Scope nat_scope.
+
 #[local] Notation "'P'" := pure.
 #[local] Notation "'BD'" := binddt.
 
@@ -347,7 +349,7 @@ consider an example where the syntax has no mutual binding structure.
               | nil => pure nil
               | cons d0 drest =>
                   pure cons <⋆> binddt_term (f ⦿ acc) d0 <⋆> F (S acc) drest
-              end) 0 defs) <⋆> binddt_term (f ⦿ List.length defs) body
+              end) 0 defs) <⋆> binddt_term (f ⦿ length defs) body
     | app t1 t2 =>
         pure (@app v2) <⋆> binddt_term f t1 <⋆> binddt_term f t2
     end.
@@ -378,7 +380,7 @@ consider an example where the syntax has no mutual binding structure.
       Lemma binddt_term_rw2: forall (l : list (term v1)) (body: term v1),
           binddt f (letin l body) =
             pure (@letin v2) <⋆> subst_in_defs f l <⋆>
-              binddt (f ⦿ List.length l) body.
+              binddt (f ⦿ length l) body.
       Proof.
         intros. cbn.
         do 2 fequal.
@@ -425,7 +427,329 @@ consider an example where the syntax has no mutual binding structure.
 
       Lemma binddt_pointfree_letin_defs: forall l,
           binddt g ∘ letin (v:=B) l =
-            (precompose (binddt (g ⦿ List.length l)) ∘ ap G2)
+            (precompose (binddt (g ⦿ length l)) ∘ ap G2)
+              (pure (letin (v:=C)) <⋆> (subst_in_defs g l)).
+      Proof.
+        intros l.
+        ext body.
+        unfold precompose, compose.
+        rewrite binddt_term_rw2.
+        reflexivity.
+      Qed.
+
+      Lemma binddt_pointfree_letin: forall `(l:list A),
+          compose (binddt g) ∘ letin (v:=B) ∘
+            mapdt_make (H := Mapdt_List_Telescope) l (B := term B) =
+            ((compose (precompose (binddt (g ⦿ length l)) ∘ ap G2) ∘
+                precompose (subst_in_defs g) ∘
+                ap G2 ∘ pure (F := G2)) (letin (v:=C))) ∘
+              mapdt_make (H := Mapdt_List_Telescope) l (B := term B).
+      Proof.
+        intros A l.
+        ext l' body.
+        unfold precompose, compose.
+        rewrite binddt_term_rw2.
+        do 2 rewrite <- list_plength_length.
+        unfold mapdt_make.
+        rewrite <- plength_trav_make.
+        reflexivity.
+      Qed.
+
+    End pointfree.
+
+  End rewriting.
+
+  #[local] Notation "'P'" := pure.
+  #[local] Notation "'BD'" := binddt.
+
+  Ltac simplify_binddt_term :=
+    match goal with
+    | |- context[BD ?f (tvar ?y)] =>
+        debug "step_BD_tvar";
+        rewrite binddt_term_rw1
+    | |- context[((BD ?f) (letin ?l ?body))] =>
+        debug "step_BD_letin";
+        rewrite binddt_term_rw2
+    | |- context[((BD ?f) (app ?t1 ?t2))] =>
+        debug "step_BD_app";
+        rewrite binddt_term_rw3
+    end.
+
+  Ltac simplify_binddt_term_lazy unit :=
+    simplify_binddt_term.
+
+(*|
+~~~~~~~~~~~~~~~~~~~~~~~~~~~~~~~~~~~~~~~~~~
+Instantiate simplification infrastructure
+~~~~~~~~~~~~~~~~~~~~~~~~~~~~~~~~~~~~~~~~~~
+|*)
+
+  Ltac derive_dtm_law :=
+    derive_dtm_law_with_simplify_binddt_IH
+      term_mut_ind2 simplify_binddt_term_lazy.
+
+  Ltac simplify_pass1 :=
+    simplify_pass1_with_simplify_binddt term simplify_binddt_term_lazy.
+
+  Ltac derive_dtm_law_case :=
+    derive_dtm_law_case_with_simplify_binddt simplify_binddt_term_lazy.
+
+  Theorem dtm1_lam:
+    forall `{Applicative G} (A B : Type),
+    forall f : nat * A -> G (term B),
+      binddt f ∘ ret  = f ∘ ret (T := (nat ×)).
+  Proof.
+    reflexivity.
+  Qed.
+
+  Theorem dtm2_term : forall A : Type,
+      binddt (T := term) (U := term)
+        (G := fun A => A) (ret (T := term) ∘ extract (W := (nat ×))) = @id (term A).
+  Proof.
+    intros.
+    derive_dtm_law.
+    derive_dtm_law_case.
+    unfold subst_in_defs.
+    unfold_ops @Mapdt_Binddt_compose.
+    apply mapdt_respectful_id.
+    intros.
+    apply ind_implies_in in H.
+    simplify_pass2.
+    eauto.
+  Qed.
+
+  Theorem dtm3_term:
+    forall `{Applicative G1} `{Applicative G2},
+    forall `(g : nat * B -> G2 (term C)) `(f : nat * A -> G1 (term B)),
+      map (binddt g) ∘ binddt f = binddt (G := G1 ∘ G2) (g ⋆7 f).
+  Proof.
+    intros. ext t.
+    generalize dependent g.
+    generalize dependent f.
+    assert (Functor G1) by (now inversion H2).
+    assert (Functor G2) by (now inversion H6).
+    unfold compose at 1.
+    induction t using term_mut_ind2; intros f g.
+    - cbn.
+      change (g ⦿ 0) with (g ⦿ Ƶ).
+      now rewrite preincr_zero.
+    - do 2 simplify_binddt_term.
+      (* left *)
+      repeat dtm3_lhs_step.
+      unfold subst_in_defs at 1;
+        unfold binddt at 2, Mapdt_Binddt_compose at 1.
+      { rewrite mapdt_repr.
+        rewrite map_to_ap.
+        repeat rewrite <- ap4;
+          repeat rewrite ap2.
+        rewrite binddt_pointfree_letin.
+        rewrite <- map_to_ap.
+        rewrite <- (fun_map_map).
+        unfold compose at 1.
+        rewrite map_to_ap.
+        rewrite <- mapdt_repr.
+        change (mapdt (A := term A) (B := term B)
+                  _ defs) with (subst_in_defs f defs).
+        (* rhs *)
+        unfold_ops @Pure_compose.
+        (* rhs defs *)
+        assert (lemma_for_defs:
+                 subst_in_defs (G := G1 ∘ G2) (g ⋆7 f) defs =
+                   map (F := G1) (subst_in_defs (G := G2) g)
+                     (subst_in_defs (G := G1) f defs)).
+        { unfold subst_in_defs.
+          unfold_ops @Mapdt_Binddt_compose.
+          compose near defs on right.
+          rewrite kdtfun_mapdt2.
+          apply mapdt_respectful.
+          - typeclasses eauto.
+          - intros w u Hin.
+            rewrite <- (kc7_preincr (G1 := G1) g f w).
+            apply ind_implies_in in Hin.
+            rewrite <- IHdefs; auto.
+            rewrite kc6_spec.
+            reflexivity.
+        }
+        Set Keyed Unification.
+        rewrite lemma_for_defs.
+        Unset Keyed Unification.
+        dtm3_rhs_applicative_compose.
+        dtm3_rhs_applicative_map.
+        (* last part *)
+        rewrite <- (kc7_preincr (G1 := G1) g f (length defs)).
+        rewrite <- IHt.
+        dtm3_rhs_applicative_compose.
+        dtm3_rhs_applicative_map.
+        reflexivity.
+      }
+    - do 2 simplify_binddt_term.
+      repeat dtm3_rhs_step.
+      dtm3_rhs_step.
+      rewrite <- IHt1.
+      dtm3_rhs_step.
+      rewrite <- IHt2.
+      dtm3_rhs_step.
+      reflexivity.
+  Qed.
+
+  Theorem dtm4_stlc :
+    forall (G1 G2 : Type -> Type) (H1 : Map G1) (H2 : Mult G1)
+      (H3 : Pure G1) (H4 : Map G2) (H5 : Mult G2) (H6 : Pure G2)
+      (ϕ : forall A : Type, G1 A -> G2 A),
+      ApplicativeMorphism G1 G2 ϕ ->
+      forall (A B : Type) (f : nat * A -> G1 (term B)),
+        ϕ (term B) ∘ binddt f = binddt (ϕ (term B) ∘ f).
+  Proof.
+    introv Happl. intros. ext t.
+    assert (Applicative G1) by (now inversion Happl).
+    assert (Applicative G2) by (now inversion Happl).
+    generalize dependent f.
+    unfold compose at 1.
+    induction t using term_mut_ind2; intro f. (* .unfold *)
+    - reflexivity.
+    - do 2 simplify_binddt_term.
+      repeat rewrite ap_morphism_1.
+      rewrite appmor_pure.
+      rewrite IHt.
+      change (ϕ (list (term B)) (subst_in_defs f defs))
+        with ((ϕ (list (term B)) ∘ subst_in_defs f) defs).
+      unfold subst_in_defs.
+      unfold_ops @Mapdt_Binddt_compose.
+      change ((?g ∘ ?f) ⦿ ?w) with (g ∘ (f ⦿ w)).
+      rewrite <- kdtfun_morph.
+      do 2 fequal.
+      apply mapdt_respectful;[typeclasses eauto|].
+      intros. cbn.
+      unfold compose.
+      apply ind_implies_in in H7.
+      apply IHdefs.
+      assumption.
+    - cbn.
+      repeat rewrite ap_morphism_1.
+      rewrite appmor_pure.
+      rewrite IHt1.
+      rewrite IHt2.
+      reflexivity.
+  Qed.
+
+End ex_binding_type2.
+
+
+Module ex_binding_type3.
+(*|
+^^^^^^^^^^^^^^^^^^^^^^^^^^^^^^^^^^^^^^^^^^^^^^^^^^^^^
+fully mutually recursive
+^^^^^^^^^^^^^^^^^^^^^^^^^^^^^^^^^^^^^^^^^^^^^^^^^^^^^
+
+To illustrate the use of the traversal representation theorem, we
+consider an example where the syntax has no mutual binding structure.
+
+|*)
+
+  Fixpoint binddt_term
+    (G : Type -> Type) `{Map G} `{Pure G} `{Mult G}
+    {v1 v2 : Type}
+    (f : nat * v1 -> G (term v2))
+    (t : term v1) : G (term v2) :=
+    match t with
+    | tvar v => f (0, v)
+    | letin defs body =>
+        pure (@letin v2) <⋆>
+        ((fix F ls :=
+            match ls with
+            | nil => pure nil
+            | cons d drest =>
+                pure cons <⋆> binddt_term (f ⦿ length defs) d <⋆> F drest
+            end) defs) <⋆> binddt_term (f ⦿ length defs) body
+    | app t1 t2 =>
+        pure (@app v2) <⋆> binddt_term f t1 <⋆> binddt_term f t2
+    end.
+
+  #[export] Instance Binddt_Lam: Binddt nat term term := @binddt_term.
+
+  Definition subst_in_defs
+    `{Applicative G} {v1 v2 : Type}
+    (f : nat * v1 -> G (term v2)):
+    list (term v1) -> G (list (term v2)) :=
+    binddt (Binddt := Mapdt_Binddt_compose (Mapdt_F := Mapdt_List_Full))
+      (U := list ∘ term) f.
+
+  Section rewriting.
+
+    Section pointful.
+
+      Context
+        `{Applicative G} (v1 v2 : Type)
+          (f : nat * v1 -> G (term v2)).
+
+      Lemma binddt_term_rw1: forall (v: v1),
+          binddt f (tvar v) = f (Ƶ, v).
+      Proof.
+        reflexivity.
+      Qed.
+
+      Lemma binddt_term_rw2: forall (l : list (term v1)) (body: term v1),
+          binddt f (letin l body) =
+            pure (@letin v2) <⋆> subst_in_defs f l <⋆>
+              binddt (f ⦿ length l) body.
+      Proof.
+        intros. cbn.
+        do 2 fequal.
+        unfold subst_in_defs.
+        unfold_ops @Mapdt_Binddt_compose.
+        unfold_ops @Mapdt_List_Full;
+          unfold mapdt_list_full.
+        match goal with
+        | |- context[(fun '(w1, t) => ?binddt (f ⦿ w1) t)] =>
+            replace (fun '(w1, t) => binddt (f ⦿ w1) t) with
+            ((fun '(w1, t) => binddt (f ⦿ w1) t) ⦿ 0)
+            by now ext [w t]
+        end.
+        match goal with
+        | |- context[BD (f ⦿ length l)] =>
+            replace (BD (f ⦿ length l)) with
+            (BD (f ⦿ (length l + 0)%nat))
+        end.
+        2: { fequal. fequal. lia. }
+        generalize dependent f; clear f.
+        generalize 0.
+        induction l; intros n f.
+        - reflexivity.
+        - cbn.
+          fequal.
+          + repeat fequal.
+            unfold_all_transparent_tcs.
+            lia.
+          + specialize (IHl (S n) f).
+            replace (length l + S n)
+              with (S (length l + n)) in IHl by lia.
+            rewrite IHl.
+            fequal.
+            ext t.
+            cbn. fequal. fequal.
+            unfold_all_transparent_tcs.
+            lia.
+      Qed.
+
+      Lemma binddt_term_rw3: forall (t1 t2: term v1),
+          binddt f (app t1 t2) =
+            pure (@app v2) <⋆> binddt f t1 <⋆> binddt f t2.
+      Proof.
+        reflexivity.
+      Qed.
+
+    End pointful.
+
+    Section pointfree.
+
+      Context
+        `{Applicative G2}
+          {B C: Type}
+          (g : nat * B -> G2 (term C)).
+
+      Lemma binddt_pointfree_letin_defs: forall l,
+          binddt g ∘ letin (v:=B) l =
+            (precompose (binddt (g ⦿ length l)) ∘ ap G2)
               (pure (letin (v:=C)) <⋆> (subst_in_defs g l)).
       Proof.
         intros l.
@@ -534,8 +858,9 @@ Instantiate simplification infrastructure
       repeat dtm3_lhs_step.
       unfold subst_in_defs at 1;
         unfold binddt at 2, Mapdt_Binddt_compose at 1.
-      #[local] Existing Instance ToBatch_Traverse.
-      { rewrite mapdt_repr.
+      { assert (ToBatch list).
+        typeclasses eauto.
+        rewrite mapdt_repr.
         rewrite map_to_ap.
         repeat rewrite <- ap4;
           repeat rewrite ap2.
@@ -629,4 +954,4 @@ Instantiate simplification infrastructure
       reflexivity.
   Qed.
 
-End ex_binding_type2.
+End ex_binding_type3.
